tests/lean/run/3029.lean
@@ -1,0 +1,12 @@
+import Lean.Data.PersistentHashMap
+open Lean
+
+example : ((PersistentHashMap.empty : PersistentHashMap Nat Nat)
+    |> (·.insert 1 1)
+    |> (·.insert 1 1)
+    |> (·.size)) = 1 := by native_decide
+
+example : ((PersistentHashMap.empty : PersistentHashMap Nat Nat)
+    |> (·.insert 1 1)
+    |> (·.insert 2 1)
+    |> (·.size)) = 2 := by native_decide
